



# DEPARTMENT OF MATHEMATICS

**[YEAR OF ESTABLISHMENT – 1997]**



# MATHEMATICS - I

**TEXT BOOK: DIFFERENTIAL CALCULUS BY  
SHANTI NARAYAN & P.K.MITTAL**

## LECTURE - 2

*Meaning of the Sign of Derivatives of  
Lagrange's mean value  
theorem(Chapter-8.3 & 8.4)*

**Ex-1:** Show that  $f(x) = x^3 - 3x^2 + 3x + 2$  is strictly increasing in every interval.

### **Solution**

We have  $f(x) = x^3 - 3x^2 + 3x + 2$  .

Then  $f'(x) = 3x^2 - 6x + 3 = 3(x-1)^2$

Thus  $f'(x) > 0$  for every value of  $x$  except one point i.e  $1$ , where it is zero.

Hence the given function is strictly increasing in every interval.

**Ex-3:** Show that

$$x/1+x < \log(1+x) < x \quad \forall x > 0$$

**Solution**

Now

$$f(x) = \log(1+x) - \frac{x}{(1+x)}, \quad x > 0$$

$$\Rightarrow f'(x) = \frac{1}{1+x} - \frac{1}{(1+x)^2} = \frac{x}{(1+x)^2}$$

$$\Rightarrow f'(x) > 0 \quad \forall x > 0 \quad \text{and is 0 for } x = 0.$$

$$\Rightarrow f \text{ is strictly increasing in } [0, \infty),$$

$$\text{Also } f(0)=0.$$

Also  $f(0)=0$ .

It follows that  $f(x) > f(0) = 0 \quad \forall x > 0$

$$\Rightarrow \log(1+x) > \frac{x}{1+x} \quad \dots(i)$$

Again  $F(x) = x - \log(1+x), \quad x > 0$

$$\Rightarrow F'(x) = 1 - \frac{1}{1+x} = \frac{x}{1+x}.$$

$\Rightarrow F'(x) > 0 \quad \forall x > 0$  and is 0 for  $x=0$ .

$\Rightarrow F(x)$  is strictly increasing in the interval  $[0, \infty)$

Also  $F(0)=0$

Thus  $F(x) > F(0) = 0 \Rightarrow x > \log(1+x) \quad \forall x > 0 \quad \dots(ii)$

Thus from (i) and (ii) we get the required result.

**Ex-5:** Show that for any  $x > 0$

$$1+x < e^x < 1+xe^x .$$

### **Solution**

Take  $f(x) = e^x - (1+x)$ . Then  $f'(x) = e^x - 1 > 0$  for any  $x > 0$ ,

So  $f$  is an increasing function and  $f(0)=0$ .

Therefore  $f > 0$  for any  $x > 0$

$$\text{i.e. } e^x - (1+x) > 0 \quad \text{or} \quad 1 + x < e^x \dots\dots\dots(1)$$

Similarly choose  $g(x) = 1 + xe^x - e^x$

Then  $g'(x) = xe^x \geq 0$  for any  $x > 0$  and  $g(0)=0$

Thus  $g$  is an increasing function and therefore  $g(x) > 0$

$$\text{i.e. } 1 + xe^x - e^x > 0 \quad \text{or} \quad e^x < 1 + xe^x \dots\dots\dots(2)$$

Results (1) and (2) form the required inequality.



**Question:** Without solving the equation prove that the equation  $x^5 + 10x + 3 = 0$  has exactly one root.

- Assume it has two solution a and b. so  $f(a)=f(b)=0$  then by Rolle's theorem for some  $c \in [a,b]$ ,  $f'(c)=0$ . but  $f'(c)=5x^4 + 10 > 0$ . hence contradiction.
- But  $f(-1)=-8$  and  $f(0)=3$ . thus there is a  $c \in [-1,0]:f(c)=0$ .
- From the two statement we prove that the equation has one real root.

The background is a solid teal color. At the top, there are several thin, wavy lines in a lighter shade of teal, creating a decorative header effect.

Thank You